

☐ The Josephus problem - Our variation

$$J(n)/w(n) = 3$$

n	w(n)
1	1
2	1
3	3
4	1
5	3
6	5
7	7
8	1
9	3
10	5
11	7
12	9
13	11
14	13
15	15
16	1

if, $n = k$
then,
 $w(n) = 1$

Ex:1
 $13 = 2^3 + (\text{Something})$
 $= 2^3 + 5$
 $= 2^k + 1$
 $= 2 \cdot 1 + 1$

Ex:2
 $41 = 2^5 + 9$
 $= 2 \cdot 1 + 1$
 $= 9 \times 2 + 1$
 $= 19$

Ex:3
 $77 = 2^6 + 13$
 $= 2 \cdot 1 + 1$
 $= 2 \times 13 + 1$
 $= 27$

Ex:4

$$77 = 2^6 \quad 2^5 \quad 2^4 \quad 2^3 \quad 2^2 \quad 2^1 \quad 2^0$$

$$1 \quad 0 \quad 0 \quad 1 \quad 1 \quad 0 \quad 1$$

$$= (0011011)_2$$

$$= (27)_{10}$$

Recurrence form:

Even: $J(2n) = 2 \cdot J(n) - 1$

Odd: $J(2n+1) = 2 \cdot J(n) + 1$

Q. Find $J(100)$ using recurrences:

Ans: $J(100) = 2 \cdot J(50) - 1$
 $= 2 \cdot \{2 \cdot J(25) - 1\} - 1$
 ~~$= 2 \cdot 2 \cdot \{2 \cdot J(12) + 1\} - 1 - 1$~~
 ~~$= 8 \cdot \{2 \cdot J(6) - 1\} + 1$~~
 $= 4 \cdot J(25) - 2 - 1$
 $= 4 \cdot \{2 \cdot J(12) + 1\} - 3$
 $= 8 \cdot J(12) + 4 - 3$
 $= 8 \cdot \{2 \cdot J(6) - 1\} + 1$

$J(100) = 16 \cdot J(6) - 8 + 1$
 $= 16 \cdot \{2 \cdot J(3) - 1\} - 7$
 $= 32 \cdot J(3) - 16 - 7$
 $= 32 \cdot \{2 \cdot J(1) + 1\} - 23$
 $= 64 \cdot J(1) + 32 - 23$
 $= 64 \times 1 + 9$

Q. Prove by induction:

Ans: $j(n) = 2l + 1$

$$\Rightarrow j(2^m + 1) = 2l + 1$$

Basis: $0 \leq l \leq 2^m$

if $m = 0, l = 0,$

$$j(2^m + 1) = 2l + 1$$

$$\Rightarrow j(2^0 + 0) = 2 \times 0 + 1$$

$$\therefore j(1) = 1 \text{ [proved]}$$

Hypothesis: Assuming from 1 to $m-1$, then equation holds:

Even: $j(2n) = 2 \cdot j(n) - 1 \text{ ----- ①}$

$$\Rightarrow 2n = 2^m + 1$$

$$\Rightarrow n = \frac{2^m + 1}{2} = \frac{2^m}{2} + \frac{1}{2} = 2^{m-1} + \frac{1}{2}$$

$$\therefore n = 2^{m-1} + \frac{1}{2}$$

(i) $j(2n) = 2 \cdot j(n) - 1$

$$= 2 \cdot j(2^{m-1} + 1/2) - 1$$

$$= 2 \cdot (2 \cdot \frac{1}{2} + 1) - 1 \quad [\because j(2^m + 1) = 2l + 1]$$

$$= 2l + 2 - 1$$

$$= 2l + 1$$

$$j(2n) = 2 \cdot j(n) - 1 \text{ ----- ①}$$

break $2n$ into the lower power of $2(2^m) + 1$

$$\therefore 2n = 2^m + 1$$

$$\Rightarrow n = (2^m + 1)/2$$

$$\Rightarrow n = \frac{2^m}{2} + \frac{1}{2}$$

$$\Rightarrow n = 2^{m-1} + \frac{1}{2}$$

$$\therefore n = 2^{m-1} + \frac{1}{2}$$

add: $j(2n+1) = 2 \cdot j(n) + 1$

$$\Rightarrow 2n+1 = 2^m + 1$$

$$\Rightarrow n = \frac{2^m + 1 - 1}{2}$$

$$\therefore n = 2^{m-1} + \frac{1-1}{2}$$

(i) $j(2n+1) = 2 \cdot j(n) + 1$

$$\Rightarrow j(2n+1) = 2 \cdot j\left(2^{m-1} + \frac{1-1}{2}\right) + 1$$

$$= 2 \cdot \left(2 \cdot \frac{1-1}{2} + 1\right) + 1$$

$$= 2 \cdot 1 + 1$$

Q. Finding values of n where $j(n) = n/3$

$$j(n) = n/3$$

$$\Rightarrow 2 \cdot 1 + 1 = \frac{2^m + 1}{3}$$

$$\Rightarrow 1 = \frac{1}{5} (2^m - 3)$$

$$2n+1 = 2^m + 1$$

$$\Rightarrow n = \frac{2^m + 1 - 1}{2}$$

$$\therefore n = 2^{m-1} + \frac{1-1}{2}$$

Probability theory and random variable

Random variable: is a function that assigns each real number to a variable from the sample space.

$$X=0 \rightarrow \text{occurrence } 1$$

$$X=1 \rightarrow \text{ " } 3$$

$$X=2 \rightarrow \text{ " } 3$$

$$X=3 \rightarrow \text{ " } 4$$

Q. 2 dice rolled ; probability of getting sum = 7

$$\rightarrow (4,3), (6,1), (5,2), (3,4), (1,6), (2,5) = 6$$

$$\therefore \text{probability} = \frac{6}{36} = \frac{1}{6}$$

Q. numbers are different

$$(1,1), (2,2), (3,3), (4,4), (5,5), (6,6) = 6 = 36 - 6 = 30$$

$$\therefore \text{probability} = \frac{30}{36} = \frac{5}{6}$$

Q. Sum of 2 fair dice,

$$P(X=2) = P(1,1) = \frac{1}{36}$$

$$P(X=3) = P\{(1,2), (2,1)\} = \frac{2}{36}$$

$$P(X=4) = P\{(1,3), (2,2), (3,1)\} = \frac{3}{36}$$

$$P(X=5) = P\{(1,4), (2,3), (3,2), (4,1)\} = \frac{4}{36}$$

$$P(X=6) = P\{(1,5), (2,4), (3,3), (4,2), (5,1)\} = \frac{5}{36}$$

Q. two coins

$$P(Y=0) = P\{(T,T)\} = \frac{1}{4}$$

$$P(Y=1) = P\{(T,H), (H,T)\} = \frac{2}{4}$$

$$P(Y=2) = P\{(H,H)\} = \frac{1}{4}$$

$$\therefore P\{Y=0\} + P\{Y=1\} + P\{Y=2\} = 1$$

Josephus Exercise:

Ex-1: given, $2l+1 = \frac{2^m+1}{2}$

$$\Rightarrow 2l = \frac{2^m+1}{2} - 1 = \frac{2^m+1-2}{2}$$

$$\Rightarrow 4l+2 = 2^m+1$$

$$\Rightarrow 4l-l+2 = 2^m$$

$$\Rightarrow 3l+2 = 2^m$$

$$\Rightarrow 3l = 2^m-2$$

$$\therefore l = \frac{1}{3} \cdot (2^m-2)$$

$$m=0; l = \frac{1}{3} (2^0-2) = 0$$

$$m=1; l = \frac{1}{3} (2^1-2) = 0; n = 2^m+l = 2+0 = 2; j(n) = 2l+1 = \frac{n}{2} = \frac{2}{2} = 1$$

$$m=2; l = \frac{1}{3} (4-2) = 2; n = 2^m+l = 6; j(n) = \frac{n}{2} = \frac{6}{2} = 3$$

$$m=3, l=10, n=42, j(n)=21$$

$$m=4, l=42, n=170, j(n)=85$$

Q. smallest 3 values of n ; person at $n/3$ position

$$\rightarrow j(n) = \frac{n}{3}$$

$$\Rightarrow 2l+1 = \frac{2^m+1}{3}$$

$$\Rightarrow 6l+3 = 2^m+1$$

$$\Rightarrow 6l-1+3 = 2^m$$

$$\Rightarrow 5l = 2^m-3$$

$$\therefore l = \frac{1}{5} \cdot (2^m-3)$$

m value: l must be int; (2^m-3) must div by 5.

$$m=1; l = \frac{1}{5} (2-3) = -1/5$$

$$m=2; l = 1/5 (4-3) = 1/5$$

$$m=3; l = 1/5 (8-3) = 5/5 = 1 \checkmark$$

$$m=7; l = 25 \checkmark$$

$$m=11; l = 409 \checkmark$$

$$\therefore n = 2^3 + 1 = 9$$

$$\therefore n = 2^7 + 25 = 153$$

$$\therefore n = 2^{11} + 409 = 2457$$

Verification:

$$j(n) = 2l+1$$

$$j(9) = 2 \times 4 + 1 = 9$$

$$j(153) = 2 \times 25 + 1 = 51$$

$$j(2457) = 2 \times 409 + 1 = 819$$

$$Q, \dot{j}(n) = 25$$

$$\Rightarrow 2l+1 = 25$$

$$\Rightarrow l = 12 \quad \therefore n = 2^m + 12$$

$$m=0; n = 2^0 + 12 = 13$$

$$m=1; n = 2^1 + 12 = 14$$

$$m=2; n = 2^2 + 12 = 16$$

$$m=3; n = 2^3 + 12 = 20 \longrightarrow \dot{j}(n) = 20 \Rightarrow 2^4 + 4 \Rightarrow 2 \times 4 + 1 = 9 \neq 25$$

$$m=4; n = 2^4 + 12 = 28 \longrightarrow \dot{j}(n) = 25 \Rightarrow 28 = 2^4 + 12 \Rightarrow 2 \times 12 + 1 = 25$$

$$m=5; n = 2^5 + 12 = 44$$

$$m=6; n = 2^6 + 12 = 76$$

$$m=7; n = 2^7 + 12 = 140$$

$$Q, \dot{j}(n) = n$$

$$\Rightarrow 2l+1 = n \Rightarrow l = \frac{n-1}{2}$$

$$\Rightarrow 2l+1 = 2^m + l \Rightarrow \boxed{l = 2^m - 1}$$

$$\therefore n = 2^m + 2^m - 1 = 2^{m+1} - 1$$

m=0	$l = 2^m - 1$	$n = 2^{m+1} - 1$	$\dot{j}(n) = n$
0	$2^0 - 1 = 1 - 1 = 0$	$2 - 1 = 1$	$2 \times 0 + 1 = 1$
1	$2^1 - 1 = 2 - 1 = 1$	$4 - 1 = 3$	$2 \times 1 + 1 = 3$
2	$2^2 - 1 = 4 - 1 = 3$	$8 - 1 = 7$	$2 \times 3 + 1 = 7$
3	$2^3 - 1 = 8 - 1 = 7$	$16 - 1 = 15$	$2 \times 7 + 1 = 15$
4	$2^4 - 1 = 16 - 1 = 15$	$32 - 1 = 31$	$2 \times 15 + 1 = 31$
5	$2^5 - 1 = 32 - 1 = 31$	$64 - 1 = 63$	$2 \times 31 + 1 = 63$